theories/Prelude/Notations.v
@@ -12,6 +12,11 @@ Reserved Infix "≦" (no associativity, at level 70).
 Reserved Infix "≨" (no associativity, at level 70).
 Reserved Infix "≺" (no associativity, at level 70).
 
+Reserved Infix "≈ₜ" (no associativity, at level 70).
+Reserved Infix "≳ₜ" (no associativity, at level 70).
+Reserved Infix "≲ₜ" (no associativity, at level 70).
+Reserved Infix "≅ₜ" (no associativity, at level 70).
+
 Reserved Infix "≦ᵣ" (no associativity, at level 70).
 Reserved Infix "=ᵣ" (no associativity, at level 70).
 Reserved Infix "<ᵣ" (no associativity, at level 70).
